src/Bedrock.v
@@ -1,6 +1,6 @@
 Require Export String List NArith.
 
-Require Export Heaps SepTheoryX SepIL.
+Require Export Heaps SepTheory SepIL.
 
 Require Export Nomega Word Memory IL LabelMap PropX PropXTac XCAP Structured StructuredModule Linker Programming.
 
