src/SepTheory.v
@@ -1,0 +1,533 @@
+Require Import Heaps Memory.
+Require Import RelationClasses.
+
+Set Implicit Arguments.
+Set Strict Implicit.
+
+Module Type SepState.
+  Parameter State : Type.
+End SepState.
+
+Module Type SepTheory.
+  Declare Module SS : SepState.
+
+  Parameter hprop : Type.
+ 
+  Parameter himp : hprop -> hprop -> Prop.
+  
+  Parameter heq : hprop -> hprop -> Prop.
+
+  Parameter Refl_himp : Reflexive himp.
+  Parameter Trans_himp : Transitive himp.
+
+  Parameter Refl_heq : Reflexive heq.
+  Parameter Sym_heq : Symmetric heq.
+  Parameter Trans_heq : Transitive heq.
+
+  Notation "a ===> b" := (himp a b) (at level 60).
+  Notation "a <===> b" := (heq a b) (at level 60).
+
+  Parameter heq_defn : forall a b, (a ===> b /\ b ===> a) <-> a <===> b.
+
+  Parameter heq_himp : forall a b, a <===> b -> a ===> b.
+
+  (* Definitions *)
+  Parameter emp : hprop.
+
+  Parameter inj : Prop -> hprop.
+
+  Parameter star : hprop -> hprop -> hprop.
+
+  Parameter ex : forall (T : Type) (p : T -> hprop), hprop.
+
+  (* star lemmas *)
+  Parameter himp_star_comm : forall P Q, 
+    (star P Q) ===> (star Q P).
+
+  Parameter heq_star_comm : forall P Q, 
+    (star P Q) <===> (star Q P).
+
+  Parameter heq_star_assoc : forall P Q R, 
+    (star (star P Q) R) <===> (star P (star Q R)).
+
+  Parameter heq_star_emp_l : forall P, (star emp P) <===> P.
+
+  Parameter heq_star_emp_r : forall P, (star P emp) <===> P.
+
+  Parameter himp_star_frame : forall P Q R S, 
+    P ===> Q -> R ===> S -> (star P R) ===> (star Q S).
+
+  Parameter heq_star_frame : forall P Q R S, 
+    P <===> Q -> R <===> S -> (star P R) <===> (star Q S).
+
+  Parameter himp_subst_p : forall P Q R S,
+    P ===> S -> (star S Q) ===> R ->
+    (star P Q) ===> R.
+
+  Parameter himp_subst_c : forall P Q R S,
+    S ===> Q -> P ===> (star S R) ->
+    P ===> (star Q R).
+
+  Parameter heq_subst : forall P Q R S,
+    P <===> S -> (star S Q) <===> R ->
+    (star P Q) <===> R.
+
+  Parameter himp_star_cancel : forall P Q R,
+    Q ===> R -> (star P Q) ===> (star P R).
+
+  Parameter heq_star_cancel : forall P Q R, 
+    Q <===> R -> (star P Q) <===> (star P R).
+
+  (** pure lemmas **)
+  Parameter himp_star_pure_p : forall P Q F,
+    (star (inj F) P) ===> Q -> (F -> P ===> Q).
+  
+  Parameter himp_star_pure_c : forall P Q (F : Prop),
+    (F -> P ===> Q) -> (star (inj F) P) ===> Q.
+
+  Parameter himp_star_pure_cc : forall P Q (p : Prop),
+    p ->
+    P ===> Q ->
+    P ===> (star (inj p) Q).
+
+  (** ex lemmas **)
+  Parameter himp_ex_p : forall T (P : T -> _) Q, 
+    (forall v, (P v) ===> Q) -> (ex P) ===> Q.
+
+  Parameter himp_ex_c : forall T (P : T -> _) Q, 
+    (exists v, Q ===> (P v)) -> Q ===> (ex P).
+
+  Parameter heq_ex : forall T (P Q : T -> _), 
+    (forall v, P v <===> Q v) ->
+    ex P <===> ex Q.
+
+  Parameter himp_ex : forall T (P Q : T -> _), 
+    (forall v, P v ===> Q v) ->
+    ex P ===> ex Q.
+
+  Parameter heq_ex_star : forall T (P : T -> _) Q,
+    (star (ex P) Q) <===> (ex (fun x => star (P x) Q)).
+
+  Parameter himp_ex_star : forall T (P : T -> _) Q,
+    (star (ex P) Q) ===> (ex (fun x => star (P x) Q)).
+
+  Existing Instance Refl_himp. 
+  Existing Instance Trans_himp. 
+  Existing Instance Refl_heq.
+  Existing Instance Sym_heq. 
+  Existing Instance Trans_heq. 
+
+End SepTheory.
+
+Module Type SepTheory_Kernel.
+  Declare Module SS : SepState.
+
+  Parameter hprop : Type.
+ 
+  Parameter himp : hprop -> hprop -> Prop.
+  
+  Parameter heq : hprop -> hprop -> Prop.
+
+  Parameter Refl_himp : Reflexive himp.
+  Parameter Trans_himp : Transitive himp.
+
+  Parameter Refl_heq : Reflexive heq.
+  Parameter Sym_heq : Symmetric heq.
+  Parameter Trans_heq : Transitive heq.
+
+  Notation "a ===> b" := (himp a b) (at level 60).
+  Notation "a <===> b" := (heq a b) (at level 60).
+
+  Parameter heq_defn : forall a b, (a ===> b /\ b ===> a) <-> a <===> b.
+  
+  (* Definitions *)
+  Parameter emp : hprop.
+
+  Parameter inj : Prop -> hprop.
+
+  Parameter star : hprop -> hprop -> hprop.
+
+  Parameter ex : forall (T : Type) (p : T -> hprop), hprop.
+
+  (* star lemmas *)
+  Parameter himp_star_comm : forall P Q, 
+    (star P Q) ===> (star Q P).
+
+  Parameter heq_star_assoc : forall P Q R, 
+    (star (star P Q) R) <===> (star P (star Q R)).
+
+  Parameter heq_star_emp_l : forall P, (star emp P) <===> P.
+
+  Parameter himp_subst_p : forall P Q R S,
+    P ===> S -> (star S Q) ===> R ->
+    (star P Q) ===> R.
+
+  Parameter himp_subst_c : forall P Q R S,
+    S ===> Q -> P ===> (star S R) ->
+    P ===> (star Q R).
+
+  (** pure lemmas **)
+  Parameter himp_star_pure_p : forall P Q F,
+    (star (inj F) P) ===> Q -> (F -> P ===> Q).
+  
+  Parameter himp_star_pure_c : forall P Q (F : Prop),
+    (F -> P ===> Q) -> (star (inj F) P) ===> Q.
+
+  Parameter himp_star_pure_cc : forall P Q (p : Prop),
+    p ->
+    P ===> Q ->
+    P ===> (star (inj p) Q).
+
+  (** ex lemmas **)
+  Parameter himp_ex_p : forall T (P : T -> _) Q, 
+    (forall v, (P v) ===> Q) -> (ex P) ===> Q.
+
+  Parameter himp_ex_c : forall T (P : T -> _) Q, 
+    (exists v, Q ===> (P v)) -> Q ===> (ex P).
+
+  Parameter heq_ex_star : forall T (P : T -> _) Q,
+    (star (ex P) Q) <===> (ex (fun x => star (P x) Q)).
+
+End SepTheory_Kernel.
+
+Module SepTheory_From_Kernel (Import K : SepTheory_Kernel) <: 
+  SepTheory with Module SS := K.SS.
+
+  Include K.
+
+  Theorem heq_himp : forall a b, a <===> b -> a ===> b.
+  Proof.
+    intros. apply heq_defn in H. intuition.
+  Qed.
+  
+  Theorem heq_star_comm : forall P Q, 
+    (star P Q) <===> (star Q P).
+  Proof.
+    intros; apply heq_defn. intuition; apply himp_star_comm.
+  Qed.
+
+  Theorem heq_star_emp_r : forall a, (star a emp) <===> a.
+  Proof.
+    intros. etransitivity. apply heq_star_comm.
+    apply heq_star_emp_l.
+  Qed.
+
+  Ltac break_heq := 
+    intros;
+      repeat match goal with
+               | [ H : _ <===> _ |- _ ] => apply heq_defn in H
+               | [ |- _ <===> _ ] => apply heq_defn
+             end; intuition.
+
+  Theorem himp_star_frame : forall P Q R S, 
+    P ===> Q -> R ===> S -> (star P R) ===> (star Q S).
+  Proof.
+    intros.
+    eapply himp_subst_p; try eassumption.
+    etransitivity.
+    eapply himp_star_comm.
+    etransitivity. 2: eapply himp_star_comm.
+    eapply himp_subst_p; try eassumption.
+    reflexivity.
+  Qed.
+
+  Theorem heq_star_frame : forall P Q R S, 
+    P <===> Q -> R <===> S -> (star P R) <===> (star Q S).
+  Proof.
+    break_heq; apply himp_star_frame; eauto.
+  Qed.
+
+  Theorem heq_subst : forall P Q R S,
+    P <===> S -> (star S Q) <===> R ->
+    (star P Q) <===> R.
+  Proof.
+    break_heq.
+    eapply himp_subst_p; try eassumption.
+    eapply himp_subst_c; try eassumption.
+  Qed.
+
+  Theorem himp_star_cancel : forall P Q R,
+    Q ===> R -> (star P Q) ===> (star P R).
+  Proof.
+    intros. etransitivity. apply himp_star_comm.
+    eapply himp_subst_p. eassumption.
+    apply himp_star_comm.
+  Qed.
+
+  Theorem heq_star_cancel : forall P Q R, 
+    Q <===> R -> (star P Q) <===> (star P R).
+  Proof.
+    break_heq.
+    apply himp_star_cancel; try eassumption.
+    apply himp_star_cancel; try eassumption.
+  Qed.
+
+  Theorem heq_ex : forall T (P Q : T -> _), 
+    (forall v, P v <===> Q v) ->
+    ex P <===> ex Q.
+  Proof.
+    break_heq;
+    apply himp_ex_p; intros; apply himp_ex_c; exists v;
+    specialize (H v); break_heq; auto.
+  Qed.    
+
+  Theorem himp_ex_star : forall T (P : T -> _) Q,
+    (star (ex P) Q) ===> (ex (fun x => star (P x) Q)).
+  Proof.
+    intros. generalize (heq_ex_star P Q).
+    break_heq.
+  Qed.
+
+  Theorem himp_ex : forall T (P Q : T -> _), 
+    (forall v, P v ===> Q v) ->
+    ex P ===> ex Q.
+  Proof.
+    intros. 
+    apply himp_ex_p; intros; apply himp_ex_c; exists v;
+    specialize (H v); break_heq; auto.
+  Qed.
+
+End SepTheory_From_Kernel.
+
+Module SepTheory_Rewrites (Import ST : SepTheory).
+  
+  Require Import Setoid Classes.Morphisms.
+  
+  Add Parametric Relation : hprop himp
+    reflexivity proved by Refl_himp
+    transitivity proved by Trans_himp
+  as himp_rel.
+
+  Add Parametric Relation : hprop heq
+    reflexivity proved by Refl_heq
+    symmetry proved by Sym_heq
+    transitivity proved by Trans_heq
+  as heq_rel.
+
+  Global Add Parametric Morphism : star with
+    signature (himp ==> himp ==> himp)
+  as star_himp_mor.
+    intros. eapply himp_star_frame; eauto.
+  Qed.
+
+  Global Add Parametric Morphism : star with
+    signature (heq ==> heq ==> heq)
+  as star_heq_mor.
+    intros. eapply heq_star_frame; eauto.
+  Qed.
+
+  Global Add Parametric Morphism T : (@ex T) with 
+    signature (pointwise_relation T (heq) ==> heq)
+  as ex_heq_mor.
+    intros. eapply heq_ex. eauto.
+  Qed.
+
+  Global Add Parametric Morphism T : (@ex T) with 
+    signature (pointwise_relation T (himp) ==> himp)
+  as ex_himp_mor.
+    intros. eapply himp_ex. auto.
+  Qed.
+
+  Global Add Parametric Morphism : (himp) with 
+    signature (heq ==> heq ==> Basics.impl)
+  as himp_heq_mor.
+    intros. intro. etransitivity.
+    symmetry in H. eapply heq_defn in H. eapply (proj1 H).
+    etransitivity. eassumption. eapply heq_defn in H0. intuition.
+  Qed.
+
+  Global Add Parametric Morphism : (himp) with 
+    signature (himp --> himp ++> Basics.impl)
+  as himp_himp_mor.
+    intros. intro. repeat (etransitivity; eauto).
+  Qed.
+
+  Global Add Parametric Morphism : inj with 
+    signature (Basics.impl ==> himp)
+  as inj_himp_mor.
+    intros.
+    intros. rewrite <- heq_star_emp_r. 
+    eapply himp_star_pure_c. intros.
+    rewrite <- heq_star_emp_r with (P := inj y).
+    eapply himp_star_pure_cc. eauto.
+    reflexivity.
+  Qed.
+
+  Global Instance subrelation_heq_himp : subrelation heq himp.
+  Proof. repeat red. apply heq_himp. Qed.
+
+  Hint Rewrite heq_star_emp_l heq_star_emp_r : hprop.
+  Existing Instance himp_rel_relation.
+  Existing Instance heq_rel_relation.
+
+End SepTheory_Rewrites.
+
+Module SepTheory_Ext (ST : SepTheory).
+  Require Import List.
+  Module Import ST_RW := SepTheory_Rewrites ST.
+  Fixpoint functionTypeD (domain : list Type) (range : Type) : Type :=
+    match domain with
+      | nil => range
+      | d :: domain' => d -> functionTypeD domain' range
+    end.
+
+  Section param.
+    Variable type : Type.
+    Variable typeD : type -> Type.
+
+    Definition existsEach (ts : list type) (f : list (@sigT _ typeD) -> ST.hprop ) 
+      : ST.hprop :=
+      @ST.ex (list (@sigT _ typeD)) (fun env => ST.star (ST.inj (map (@projT1 _ _) env = ts)) (f env)).
+
+    Ltac thinker := 
+      repeat match goal with
+               | [ H : forall f, ST.himp _ _ _ |- _ ] => rewrite H
+               | [ |- _ ] => reflexivity
+               | [ |- ST.himp (ST.star (ST.inj _) _) _ ] => 
+                 apply ST.himp_star_pure_c ; intros
+               | [ |- ST.himp (ST.ex _) _ ] => 
+                 apply ST.himp_ex_p ; intros
+               | [ |- ST.himp _ (ST.ex (fun x => ST.star (ST.inj (?X = _)) _)) ] => 
+                 apply ST.himp_ex_c ; exists nil ; eapply ST.himp_star_pure_cc; [ solve [ eauto ] | ]
+               | [ |- ST.himp _ (ST.ex (fun x => ST.star (ST.inj (?X = _)) _)) ] => 
+                 apply ST.himp_ex_c ; eexists; eapply ST.himp_star_pure_cc; [ solve [ eauto ] | ]
+             end.
+
+    Lemma existsEach_perm : forall (F : list (@sigT _ typeD) -> _) x x',
+        ST.heq (existsEach x (fun e => existsEach x' (fun e' => F (e ++ e'))))
+               (existsEach x' (fun e' => existsEach x (fun e => F (e ++ e')))).
+    Proof.
+      intros. eapply ST.heq_defn. split; unfold existsEach;
+      revert F; revert x'; induction x; simpl; intros;
+        repeat match goal with
+                 | [ H : forall f, ST.himp _ _ |- _ ] => rewrite H
+                 | [ |- _ ] => reflexivity
+                 | [ |- ST.himp (ST.star (ST.inj _) _) _ ] => 
+                   apply ST.himp_star_pure_c ; intros
+                 | [ |- ST.himp (ST.ex _) _ ] => 
+                   apply ST.himp_ex_p ; intros
+                 | [ |- ST.himp _ (ST.ex (fun x => ST.star (ST.inj (?X = _)) _)) ] => 
+                   apply ST.himp_ex_c ; eexists; eapply ST.himp_star_pure_cc; [ solve [ eauto ] | ]
+               end.
+    Qed.
+
+    Lemma map_eq_app : forall T U (F : T -> U) ls x y,
+      map F ls = x ++ y ->
+      exists x' y', ls = x' ++ y' /\ map F x' = x /\ map F y' = y.
+    Proof.
+      clear. induction ls; destruct x; simpl in *; intros; subst; try congruence.
+      exists nil; exists nil; simpl; auto.
+      exists nil. simpl. eexists; eauto.
+      inversion H; clear H; subst. eapply IHls in H2.
+      destruct H2. destruct H. intuition. subst. exists (a :: x0). exists x1. simpl; eauto.
+    Qed.
+    
+    Lemma existsEach_app : forall x x' (F : list (@sigT _ typeD) -> _) ,
+      ST.heq (existsEach (x ++ x') F)
+             (existsEach x (fun e => existsEach x' (fun e' => F (e ++ e')))).
+    Proof.
+      intros. eapply ST.heq_defn. split; unfold existsEach;
+      revert F; revert x'; induction x; simpl; intros; thinker.
+      Focus 2. destruct v; simpl in *; try congruence; reflexivity.
+      Focus 2. apply ST.himp_ex_c ; eexists (v ++ v0); eapply ST.himp_star_pure_cc. rewrite map_app. rewrite H. rewrite H0. auto.
+      reflexivity.
+      change (a :: x ++ x') with ((a :: x) ++ x') in H.
+      eapply map_eq_app in H. do 2 destruct H. intuition; subst. thinker.
+    Qed.
+
+    Lemma existsEach_nil : forall (F : list (@sigT _ typeD) -> _) ,
+      ST.heq (existsEach nil F) (F nil).
+    Proof.
+      intros. eapply ST.heq_defn. unfold existsEach; split; thinker.
+      destruct v; try reflexivity. simpl in *; congruence.
+    Qed.
+
+    Lemma heq_existsEach : forall x (F F' : list (@sigT _ typeD) -> _) ,
+      (forall G, map (@projT1 _ _) G = x -> ST.heq (F G) (F' G)) ->
+      ST.heq (existsEach x F) (existsEach x F').
+    Proof.
+      intros. eapply ST.heq_ex. intros. apply ST.heq_defn. split; thinker;
+      eapply ST.himp_star_pure_cc; eauto; specialize (H _ H0); apply ST.heq_defn in H; intuition.
+    Qed.
+
+    Lemma himp_existsEach : forall x (F F' : list (@sigT _ typeD) -> _) ,
+      (forall G, map (@projT1 _ _) G = x -> ST.himp (F G) (F' G)) ->
+      ST.himp (existsEach x F) (existsEach x F').
+    Proof.
+      intros. eapply ST.himp_ex. intros. thinker;
+      eapply ST.himp_star_pure_cc; eauto; specialize (H _ H0); apply ST.heq_defn in H; intuition.
+    Qed.
+
+    Lemma himp_existsEach_p : forall x (F : list (@sigT _ typeD) -> _) F',
+      (forall G, map (@projT1 _ _) G = x -> ST.himp (F G) F') ->
+      ST.himp (existsEach x F) F'.
+    Proof.
+      intros. eapply ST.himp_ex_p. intros. eapply ST.himp_star_pure_c. intros.
+      eapply H; eauto.
+    Qed.
+
+    Lemma himp_existsEach_c : forall x (F : list (@sigT _ typeD) -> _) F',
+      (exists G, map (@projT1 _ _) G = x /\ ST.himp F' (F G)) ->
+      ST.himp F' (existsEach x F).
+    Proof.
+      intros. eapply ST.himp_ex_c. intros. destruct H.
+      exists x0. intuition. rewrite H1. eapply ST.himp_star_pure_cc; auto. reflexivity. 
+    Qed.
+
+    Lemma heq_pushIn : forall P x (F : list (@sigT _ typeD) -> _) ,
+      ST.heq (ST.star P (existsEach x F)) (existsEach x (fun e => ST.star P (F e))).
+    Proof.
+      intros. unfold existsEach; intros.
+      rewrite ST.heq_star_comm. rewrite ST.heq_ex_star. eapply ST.heq_ex. intros. 
+      repeat rewrite ST.heq_star_assoc. eapply ST.heq_defn; split; thinker; eapply ST.himp_star_pure_cc; eauto.
+      rewrite ST.heq_star_comm. reflexivity.
+      rewrite ST.heq_star_comm. reflexivity.
+    Qed.
+    
+    Lemma existsEach_cons : forall v vs P,
+      ST.heq (existsEach (v :: vs) P)
+             (ST.ex (fun x => existsEach vs (fun env => P (@existT _ _ v x :: env)))).
+    Proof.
+      intros. change (v :: vs) with ((v :: nil) ++ vs). rewrite existsEach_app.
+      eapply ST.heq_defn. simpl. split; unfold existsEach; thinker. eapply ST.himp_ex_c. 
+      destruct v0; simpl in *; try congruence.
+      inversion H; clear H; subst. exists (projT2 s). destruct v0; simpl in *; try congruence.
+      eapply ST.himp_ex_c. exists v1. eapply ST.himp_star_pure_cc; eauto. destruct s; simpl; reflexivity.
+
+      eapply ST.himp_ex_c. exists (existT typeD v v0 :: nil). simpl. eapply ST.himp_star_pure_cc; eauto. 
+      eapply ST.himp_ex_c. exists v1. eapply ST.himp_star_pure_cc; eauto. reflexivity.
+    Qed.
+
+    Lemma existsEach_rev : forall v F,
+      ST.heq (existsEach v F) (existsEach (rev v) (fun e => F (rev e))).
+    Proof.
+      intros; eapply ST.heq_defn; split; revert F; induction v; simpl; intros;
+        repeat (rewrite existsEach_nil || rewrite existsEach_cons || rewrite existsEach_app); unfold existsEach; thinker; auto.
+      { apply ST.himp_ex_c. exists (rev v1). apply ST.himp_star_pure_cc. subst. rewrite map_rev. reflexivity.
+        apply ST.himp_ex_c. exists (@existT _ _ a v0 :: nil). apply ST.himp_star_pure_cc. reflexivity.
+        rewrite rev_app_distr. rewrite rev_involutive. reflexivity. }
+      { eapply ST.himp_ex_c. destruct v1. simpl in *; congruence. simpl in *. destruct s; simpl in *.
+        inversion H0; clear H0; subst. exists t. rewrite rev_app_distr. simpl. rewrite app_ass. simpl.
+        apply ST.himp_ex_c. exists (rev v0). apply ST.himp_star_pure_cc. rewrite map_rev. rewrite H. apply rev_involutive.
+        destruct v1; try reflexivity. simpl in *; congruence. }
+    Qed.
+
+(*
+    Lemma interp_existsEach : forall vs P stn st,
+      ST.satisfies (existsEach vs P) stn st ->
+      exists G, map (@projT1 _ _) G = vs /\ ST.satisfies cs (P G) stn st. 
+    Proof.
+      intros. apply ST.satisfies_ex in H. destruct H. exists x.
+      apply ST.satisfies_star in H. 
+      repeat match goal with
+               | [ H : exists x, _ |- _ ] => destruct H
+               | [ H : _ /\ _ |- _ ] => destruct H
+             end.
+      apply ST.satisfies_pure in H0. intuition.
+      PropXTac.propxFo. eapply ST.HT.split_semp in H; eauto. subst; auto.
+    Qed.
+*)
+
+  End param.
+End SepTheory_Ext.
+
